src/arithmetic.lean
@@ -1,0 +1,47 @@
+import deduction
+
+open language
+
+inductive langf : ℕ → Type
+| zero : langf 0
+| succ : langf 1
+| add  : langf 2
+| mult : langf 2
+
+inductive langp : ℕ → Type
+| le : langp 2
+
+def AL : language := ⟨langf, langp⟩
+
+notation `Ż` := AL.symbolf₀ langf.zero
+
+prefix `Ṡ`:max := AL.symbolf₁ langf.succ
+
+infixl ` +̇ `:92 := AL.symbolf₂ langf.add
+
+infixl ` ×̇ `:92 := AL.symbolf₂ langf.mult
+
+infixl ` ≤̇ `:90 := (AL.symbolp₂ langp.le)
+
+def numeral : ℕ → AL.term
+| 0     := Ż
+| (n+1) := Ṡ(numeral n)
+
+local prefix `˙`:max := numeral
+
+inductive Q : AL.theory
+| ax1 : Q Ȧ(˙0 ≠̇ #0)
+| ax2 : Q ȦȦ(Ṡ #0 =̇ Ṡ #1 →̇ #0 =̇ #1)
+| ax3 : Q Ȧ(#0 ≠̇ ˙0 →̇ Ė(#1 =̇ Ṡ #0))
+| ax4 : Q Ȧ(˙0 +̇ #0 =̇ #0)
+| ax5 : Q ȦȦ((Ṡ #0) +̇ #1 =̇ Ṡ(#0 +̇ #1))
+| ax6 : Q Ȧ(˙0 ×̇ #0 =̇ ˙0)
+| ax7 : Q ȦȦ((Ṡ #0) ×̇ #1 =̇ (#0 +̇ #1) +̇ #1)
+| ax8 : Q ȦȦ(#0 ≤̇ #1 →̇ Ė(#1 +̇ #0 =̇ #2))
+
+
+#reduce ˙2 +̇ ˙3
+
+#check AL.symbolp₂ langp.le
+
+#check (AL.symbolp₂ langp.le)
