src/deduction.lean
@@ -17,26 +17,26 @@ inductive provable : L.theory → L.form → Prop
 | mp  : ∀ {T : theory L} {p q}, provable T (p →̇ q) → provable T p → provable T q
 | ax  : ∀ {T : theory L} {p}, T p → provable T p
 | p1  : ∀ (T : theory L) (p q), provable T (p →̇ q →̇ p)
-| p2  : ∀ (T : theory L) (p q r), provable T ((p →̇ q →̇ r) →̇ ((p →̇ q) →̇ (p →̇ r)))
-| p3  : ∀ (T : theory L) (p q), provable T ((¬̇ p →̇ ¬̇ q) →̇ (q →̇ p))
-| q1  : ∀ (T : theory L) (p t), provable T ((Ȧ p) →̇ p.(t))
-| q2  : ∀ (T : theory L) (p q), provable T ((Ȧ p →̇ q) →̇ (Ȧ p) →̇ Ȧ q)
+| p2  : ∀ (T : theory L) (p q r), provable T ((p →̇ q →̇ r) →̇ (p →̇ q) →̇ p →̇ r)
+| p3  : ∀ (T : theory L) (p q), provable T ((¬̇ p →̇ ¬̇ q) →̇ q →̇ p)
+| q1  : ∀ (T : theory L) (p t), provable T (Ȧ p →̇ p.(t))
+| q2  : ∀ (T : theory L) (p q), provable T (Ȧ (p →̇ q) →̇ Ȧ p →̇ Ȧ q)
 | q3  : ∀ (T : theory L) (p), provable T (p →̇ Ȧ p.sf)
 | e1  : ∀ (T : theory L) (t), provable T (t =̇ t)
 | e2  : ∀ (T : theory L) (p : L.form) (t u), provable T (t =̇ u →̇ p.(t) →̇ p.(u))
 
-infix ` ⊢̌ `:60 := provable
+infix ` ⊢̇ `:60 := provable
 
 attribute [simp] provable.p1 provable.p2 provable.p3 provable.q1 provable.q2 provable.q3
   provable.e1 provable.e2
 
-def theory.consistent (T : L.theory) : Prop := ¬∃p, (T ⊢̌ p) ∧ (T ⊢̌ ¬̇p) 
+def theory.consistent (T : L.theory) : Prop := ¬∃p, (T ⊢̇ p) ∧ (T ⊢̇ ¬̇p) 
 
 inductive theory.add (T : L.theory) (p : L.form) : L.theory 
 | new : theory.add p
 | old : ∀ {q}, T q → theory.add q
 
-infixl ` ¦ `:max := theory.add
+infixl ` ¦ `:60 := theory.add
 
 def theory.delete (T : L.theory) (p : L.form) : L.theory := λ q, T q ∧ q ≠ p
 
@@ -47,20 +47,30 @@ instance : has_subset L.theory := ⟨theory.include⟩
 namespace provable
 variables (T : L.theory)
 
-@[simp] lemma pp (p) : T ⊢̌ p →̇ p :=
-by { have l₀ : T ⊢̌ (p →̇ (p →̇ p) →̇ p) →̇ (p →̇ p →̇ p) →̇ p →̇ p, simp,
-     have l₁ : T ⊢̌ p →̇ (p →̇ p) →̇ p, simp,
-     have l₂ : T ⊢̌ (p →̇ p →̇ p) →̇ p →̇ p, refine l₀.mp l₁,
-     have l₃ : T ⊢̌ p →̇ p →̇ p, simp,
-     refine l₂.mp l₃ }
-
-lemma imp_r {p} (h : T ⊢̌ p) (q) : T ⊢̌ q →̇ p :=
-by { have : T ⊢̌ p →̇ q →̇ p, simp,
-     exact this.mp h }
+@[simp] lemma pp (p) : T ⊢̇ p →̇ p :=
+begin
+  have l₀ : T ⊢̇ (p →̇ (p →̇ p) →̇ p) →̇ (p →̇ p →̇ p) →̇ p →̇ p, simp,
+  have l₁ : T ⊢̇ p →̇ (p →̇ p) →̇ p, simp,
+  have l₂ : T ⊢̇ (p →̇ p →̇ p) →̇ p →̇ p, refine l₀.mp l₁,
+  have l₃ : T ⊢̇ p →̇ p →̇ p, simp,
+  refine l₂.mp l₃
+end
 
 variables {T}
 
-lemma inclusion {p} (h : T ⊢̌ p) : ∀ {U}, T ⊆ U → U ⊢̌ p :=
+@[simp] lemma imp_r {p} (h : T ⊢̇ p) (q) : T ⊢̇ q →̇ p :=
+by { have : T ⊢̇ p →̇ q →̇ p, simp,
+     exact this.mp h }
+
+lemma imp_trans {p q r} : (T ⊢̇ p →̇ q) → (T ⊢̇ q →̇ r) → (T ⊢̇ p →̇ r) := λ h₁ h₂,
+begin
+  have l₁ : T ⊢̇ (p →̇ q →̇ r) →̇ (p →̇ q) →̇ (p →̇ r), simp,  
+  have l₂ : T ⊢̇ (p →̇ q →̇ r), simp[h₂],
+  have l₃ : T ⊢̇ (p →̇ q) →̇ (p →̇ r), from l₁.mp l₂,
+  exact l₃.mp h₁
+end
+
+lemma inclusion {p} (h : T ⊢̇ p) : ∀ {U}, T ⊆ U → U ⊢̇ p :=
 begin
   induction h with T p hyp_p IH T p q hyp_pq hyp_p IH₁ IH₂ T p hyp_p; try { simp },
   { intros U hyp, refine gen (IH (λ x h, _)), cases h with p hp,
@@ -69,10 +79,37 @@ begin
   { intros U hyp, exact ax (hyp _ hyp_p) }
 end
 
-lemma weakening (p) {q} : T ⊢̌ q → T ¦ p ⊢̌ q := λ hyp,
-inclusion hyp (λ x h, theory.add.old h)
+@[simp] lemma weakening {q} (h : T ⊢̇ q) (p) : T ¦ p ⊢̇ q :=
+inclusion h (λ x h, theory.add.old h)
 
-theorem deduction {p q} : T ¦ p ⊢̌ q → T ⊢̌ p →̇ q :=
+private lemma delete_imply {p} (h : T ⊢̇ p) : ∀ q, (T.delete q) ⊢̇ q →̇ p :=
+begin
+  induction h with T p hyp_p IH T p₁ p₂ hyp_p₁₂ hyp_p₁ IH₁ IH₂ T p hyp_p;
+    try { intros q, apply imp_r, simp }; intros q,
+  { have IH : (⇑T).delete q.sf ⊢̇ q.sf →̇ p := IH q.sf,
+    have lmm₁ : T.delete q ⊢̇ q →̇ Ȧ q.sf, { simp },
+    have lmm₂ : T.delete q ⊢̇ Ȧ q.sf →̇ Ȧ p,
+    { suffices : T.delete q ⊢̇ Ȧ (q.sf →̇ p),
+      { have lmm : T.delete q ⊢̇ Ȧ(q.sf →̇ p) →̇ Ȧ q.sf →̇ Ȧ p, simp,
+        exact lmm.mp this },
+      refine gen (inclusion IH (λ x h, _)), 
+      rcases h with ⟨h, neq⟩, rcases h with ⟨p', h'⟩,
+      refine theory.sf.intro ⟨h', λ c, _⟩,
+      rw c at neq, exact neq rfl },
+    exact lmm₁.imp_trans lmm₂ },
+  { have : T.delete q ⊢̇ (q →̇ p₁ →̇ p₂) →̇ (q →̇ p₁) →̇ (q →̇ p₂), simp, 
+    have : T.delete q ⊢̇ (q →̇ p₁) →̇ q →̇ p₂, from this.mp (IH₁ _),
+    exact this.mp (IH₂ _) },
+  { by_cases eqn : p = q,
+    { simp[eqn] },
+    { have : T.delete q ⊢̇ p, from ax ⟨hyp_p, eqn⟩,
+      simp[this] } }
+end
+
+theorem deduction {p q} : (T ¦ p ⊢̇ q) → (T ⊢̇ p →̇ q) := λ h,
+by { have : (T ¦ p).delete p ⊢̇ p →̇ q, from delete_imply h p,
+     refine inclusion this (λ x h, _), rcases h with ⟨h, neq⟩,
+     cases h; simp* at* }
 
 
 end provable
